src/HeapState.v
@@ -80,7 +80,7 @@ Proof.
   apply H0; nomega.
 Qed.
 
-Definition find_free_block (len : Size) (r : M.t Ptr) : Comp Ptr :=
+Definition find_free_block (len : Size) `(r : M.t (Ptr A)) : Comp (Ptr A) :=
   { addr : N | P.for_all (fun a sz => negb (overlaps_bool a sz addr len)) r }.
 
 Definition keep_range {elt} (addr : M.key) (len : N) : M.t elt -> M.t elt :=
