src/Memory.v
@@ -2,7 +2,7 @@ Require Import
   Coq.NArith.NArith
   Coq.Strings.Ascii.
 
-Definition Ptr  := N.
+Definition Ptr (A : Type) := N.
 Definition Size := N.
 Definition Word := Ascii.ascii.
 Definition Zero := Ascii.zero.
